wstep_comp_op

nondeterministic_dataflow/Wstep_Composition.thy
@@ -4,6 +4,244 @@ imports
   "BNA_Operators"
 begin
 
+
+inductive wstep_comp_op where
+  \<open>comp_op wire buf' op1' op2' = comp_op wire buf op1 op2 \<Longrightarrow> wstep_comp_op Tau wire buf buf' op1 op1' op2 op2'\<close>
+| \<open>step Tau op1 op1' \<Longrightarrow> wstep_comp_op Tau wire buf buf' op1' op1'' op2 op2' \<Longrightarrow> wstep_comp_op Tau wire buf buf' op1 op1'' op2 op2'\<close>
+| \<open>step Tau op2 op2' \<Longrightarrow> wstep_comp_op Tau wire buf buf' op1 op1' op2' op2'' \<Longrightarrow> wstep_comp_op Tau wire buf buf' op1 op1' op2 op2''\<close>
+| \<open>wstep_comp_op Tau wire buf buf' op1 op1' op2 op2' \<Longrightarrow> step (Inp p x) op1' op1'' \<Longrightarrow> wstep_comp_op Tau wire buf' buf'' op1'' op1''' op2' op2'' \<Longrightarrow> wstep_comp_op (Inp (Inl p) x) wire buf buf'' op1 op1''' op2 op2''\<close>
+| \<open>wstep_comp_op Tau wire buf buf' op1 op1' op2 op2' \<Longrightarrow>step (Out p x) op2' op2'' \<Longrightarrow> wstep_comp_op Tau wire buf' buf'' op1' op1'' op2'' op2''' \<Longrightarrow> wstep_comp_op (Out (Inr p) x) wire buf buf'' op1 op1'' op2 op2'''\<close>
+| \<open>wstep_comp_op Tau wire buf buf' op1 op1' op2 op2' \<Longrightarrow> step (Out p x) op1' op1'' \<Longrightarrow> wire p = None \<Longrightarrow> wstep_comp_op Tau wire buf' buf'' op1'' op1''' op2' op2'' \<Longrightarrow> wstep_comp_op (Out (Inl p) x) wire buf buf'' op1 op1''' op2 op2''\<close>
+| \<open>wstep_comp_op Tau wire buf buf' op1 op1' op2 op2' \<Longrightarrow> step (Inp p x) op2' op2'' \<Longrightarrow> p \<notin> ran wire \<Longrightarrow> wstep_comp_op Tau wire buf' buf'' op1' op1'' op2'' op2''' \<Longrightarrow> wstep_comp_op (Inp (Inr p) x) wire buf buf'' op1 op1'' op2 op2'''\<close>
+| \<open>step (Out p x) op1 op1' \<Longrightarrow> wire p = Some q \<Longrightarrow> wstep_comp_op Tau wire (BENQ q x buf) buf'' op1' op1'' op2 op2' \<Longrightarrow> wstep_comp_op Tau wire buf buf'' op1 op1'' op2 op2'\<close>
+| \<open>step (Inp p x) op2 op2' \<Longrightarrow> p \<in> ran wire \<Longrightarrow> buf p \<noteq> [] \<Longrightarrow> BHD p buf = x \<Longrightarrow> wstep_comp_op Tau wire (BTL p buf) buf'' op1 op1' op2' op2'' \<Longrightarrow> wstep_comp_op Tau wire buf buf'' op1 op1' op2 op2''\<close>
+
+lemma step_Taus_comp_op:
+  \<open>(step Tau)\<^sup>*\<^sup>* (comp_op wire buf op1 op2) (comp_op wire buf' op1' op2') \<Longrightarrow> wstep_comp_op Tau wire buf buf' op1 op1' op2 op2'\<close>
+  apply (induct "comp_op wire buf op1 op2" arbitrary: buf op1 op2 rule: converse_rtranclp_induct)
+   apply (auto intro: wstep_comp_op.intros elim!: step_comp_op_elim)
+  done
+
+lemma wstep_comp_op:
+  \<open>wstep io (comp_op wire buf op1 op2) (comp_op wire buf' op1' op2') \<longleftrightarrow> wstep_comp_op io wire buf buf' op1 op1' op2 op2'\<close>
+  apply (rule iffI)
+  subgoal
+    unfolding wstep_def
+    apply (erule relcomppE)
+    subgoal for op
+      apply (induct "comp_op wire buf op1 op2" arbitrary: buf op1 op2  rule: converse_rtranclp_induct)
+      subgoal 
+        apply (cases io; simp)
+        subgoal for p x
+          apply (cases p)
+          subgoal
+            apply hypsubst_thin
+            apply (erule relcomppE)
+            apply (auto intro: step_Taus_comp_op wstep_comp_op.intros elim!: step_comp_op_elim)
+            done
+          subgoal
+            apply hypsubst_thin
+            apply (erule relcomppE)
+            apply (auto intro: step_Taus_comp_op wstep_comp_op.intros elim!: step_comp_op_elim)
+            done
+          done
+        subgoal
+          apply hypsubst_thin
+          apply (erule relcomppE)
+          apply (auto intro: step_Taus_comp_op wstep_comp_op.intros elim!: step_comp_op_elim)
+          done
+        subgoal
+          apply hypsubst_thin
+          apply (smt (verit, best) converse_rtranclp_into_rtranclp pick_middlep step_Taus_comp_op)
+          done
+        done
+      subgoal for op buf op1 op2
+        apply (cases io; simp)
+        subgoal for p x
+          apply (cases p)
+          subgoal for p
+            apply hypsubst_thin
+            apply (erule relcomppE)
+            subgoal for op''
+              apply (auto intro: step_Taus_comp_op wstep_comp_op.intros elim!: step_comp_op_elim)
+                 apply hypsubst_thin
+              subgoal
+                apply (drule meta_spec)+
+                apply (drule meta_mp)
+                 apply (rule refl)
+                apply (erule wstep_comp_op.cases)
+                        apply (auto intro: step_Taus_comp_op wstep_comp_op.intros elim!: step_comp_op_elim)
+                done
+              subgoal
+                apply (drule meta_spec)+
+                apply (drule meta_mp)
+                 apply (rule refl)
+                apply (erule wstep_comp_op.cases)
+                        apply (auto intro: step_Taus_comp_op wstep_comp_op.intros elim!: step_comp_op_elim)
+                done
+              subgoal
+                apply (drule meta_spec)+
+                apply (drule meta_mp)
+                 apply (rule refl)
+                apply (erule wstep_comp_op.cases)
+                        apply (auto intro: step_Taus_comp_op wstep_comp_op.intros elim!: step_comp_op_elim)
+                done
+              subgoal
+                apply (drule meta_spec)+
+                apply (drule meta_mp)
+                 apply (rule refl)
+                apply (erule wstep_comp_op.cases)
+                        apply (auto intro: step_Taus_comp_op wstep_comp_op.intros elim!: step_comp_op_elim)
+                done
+              done
+            done
+          subgoal for p
+            apply hypsubst_thin
+            apply (erule relcomppE)
+            subgoal for op''
+              apply (auto intro: step_Taus_comp_op wstep_comp_op.intros elim!: step_comp_op_elim)
+                 apply hypsubst_thin
+              subgoal
+                apply (drule meta_spec)+
+                apply (drule meta_mp)
+                 apply (rule refl)
+                apply (erule wstep_comp_op.cases)
+                        apply (auto intro: step_Taus_comp_op wstep_comp_op.intros elim!: step_comp_op_elim)
+                done
+              subgoal
+                apply (drule meta_spec)+
+                apply (drule meta_mp)
+                 apply (rule refl)
+                apply (erule wstep_comp_op.cases)
+                        apply (auto intro: step_Taus_comp_op wstep_comp_op.intros elim!: step_comp_op_elim)
+                done
+              subgoal
+                apply (drule meta_spec)+
+                apply (drule meta_mp)
+                 apply (rule refl)
+                apply (erule wstep_comp_op.cases)
+                        apply (auto intro: step_Taus_comp_op wstep_comp_op.intros elim!: step_comp_op_elim)
+                done
+              subgoal
+                apply (drule meta_spec)+
+                apply (drule meta_mp)
+                 apply (rule refl)
+                apply (erule wstep_comp_op.cases)
+                        apply (auto intro: step_Taus_comp_op wstep_comp_op.intros elim!: step_comp_op_elim)
+                done
+              done
+            done
+          done
+        subgoal for p x
+          apply (cases p)
+          subgoal for p
+            apply hypsubst_thin
+            apply (erule relcomppE)
+            subgoal for op''
+              apply (auto intro: step_Taus_comp_op wstep_comp_op.intros elim!: step_comp_op_elim)
+                 apply hypsubst_thin
+              subgoal
+                apply (drule meta_spec)+
+                apply (drule meta_mp)
+                 apply (rule refl)
+                apply (erule wstep_comp_op.cases)
+                        apply (auto intro: step_Taus_comp_op wstep_comp_op.intros elim!: step_comp_op_elim)
+                done
+              subgoal
+                apply (drule meta_spec)+
+                apply (drule meta_mp)
+                 apply (rule refl)
+                apply (erule wstep_comp_op.cases)
+                        apply (auto intro: step_Taus_comp_op wstep_comp_op.intros elim!: step_comp_op_elim)
+                done
+              subgoal
+                apply (drule meta_spec)+
+                apply (drule meta_mp)
+                 apply (rule refl)
+                apply (erule wstep_comp_op.cases)
+                        apply (auto intro: step_Taus_comp_op wstep_comp_op.intros elim!: step_comp_op_elim)
+                done
+              subgoal
+                apply (drule meta_spec)+
+                apply (drule meta_mp)
+                 apply (rule refl)
+                apply (erule wstep_comp_op.cases)
+                        apply (auto intro: step_Taus_comp_op wstep_comp_op.intros elim!: step_comp_op_elim)
+                done
+              done
+            done
+          subgoal for p
+            apply hypsubst_thin
+            apply (erule relcomppE)
+            subgoal for op''
+              apply (auto intro: step_Taus_comp_op wstep_comp_op.intros elim!: step_comp_op_elim)
+                 apply hypsubst_thin
+              subgoal
+                apply (drule meta_spec)+
+                apply (drule meta_mp)
+                 apply (rule refl)
+                apply (erule wstep_comp_op.cases)
+                        apply (auto intro: step_Taus_comp_op wstep_comp_op.intros elim!: step_comp_op_elim)
+                done
+              subgoal
+                apply (drule meta_spec)+
+                apply (drule meta_mp)
+                 apply (rule refl)
+                apply (erule wstep_comp_op.cases)
+                        apply (auto intro: step_Taus_comp_op wstep_comp_op.intros elim!: step_comp_op_elim)
+                done
+              subgoal
+                apply (drule meta_spec)+
+                apply (drule meta_mp)
+                 apply (rule refl)
+                apply (erule wstep_comp_op.cases)
+                        apply (auto intro: step_Taus_comp_op wstep_comp_op.intros elim!: step_comp_op_elim)
+                done
+              subgoal
+                apply (drule meta_spec)+
+                apply (drule meta_mp)
+                 apply (rule refl)
+                apply (erule wstep_comp_op.cases)
+                        apply (auto intro: step_Taus_comp_op wstep_comp_op.intros elim!: step_comp_op_elim)
+                done
+              done
+            done
+          done
+        subgoal
+          by (auto intro: step_Taus_comp_op wstep_comp_op.intros elim!: step_comp_op_elim)
+        done
+      done
+    done
+  subgoal
+    apply (induct pred: wstep_comp_op)
+            apply force
+           apply blast
+          apply blast
+    subgoal for wire buf buf' op1 op1' op2 op2' p x op1'' buf'' op1''' op2''
+      apply simp
+      apply (smt (verit, ccfv_threshold) estep.simps(2) relcompp_apply step_comp_op_L_Inp wstep_def)
+      done
+    subgoal for wire buf buf' op1 op1' op2 op2' p x op2'' buf'' op1'' op2'''
+      apply simp
+      apply (smt (verit, best) estep.simps(3) relcomppI step_comp_op_R_Out wstep_def)
+      done
+    subgoal
+      apply simp
+      apply (smt (verit, ccfv_threshold) domIff estep.simps(3) relcomppI step_comp_op_L_Out wstep_def)
+      done
+    subgoal
+      apply simp
+      apply (smt (verit, best) estep.simps(2) relcompp_apply step_comp_op_R_Inp wstep_def)
+      done
+    subgoal
+      apply simp
+      apply (meson converse_rtranclp_into_rtranclp step_Tau_comp_op_L_alt)
+      done
+    subgoal
+      by blast
+    done
+  done
+
 inductive wstep_comp_op_L where
   \<open>io = Tau \<Longrightarrow> buf = (\<lambda>_. []) \<Longrightarrow> op' = op \<Longrightarrow> wstep_comp_op_L io wire buf op op'\<close>
 | \<open>io = Inp (Inl p) x \<Longrightarrow> step (Inp p x) op op' \<Longrightarrow> wstep_comp_op_L Tau wire buf op' op'' \<Longrightarrow>
